Add proofs for requirement 8 for program "Massage chair"

MassageChair/Requirements.thy
@@ -1,5 +1,5 @@
 theory Requirements
-  imports MassageChair "../Pattern1_Def" "../Pattern6_Def" "../Pattern12_Def" "../Pattern3_Def"
+  imports MassageChair "../Pattern1_Def" "../Pattern6_Def" "../Pattern12_Def" "../Pattern2_Def"
 begin
 
 definition R1 where "R1 s \<equiv> toEnvP s \<and>
@@ -32,9 +32,9 @@ definition R7 where "R7 s \<equiv> toEnvP s \<and>
 getVarBool s2 roller' = False \<and> getVarBool s2 vibration' = False)"
 
 definition R7_1 where "R7_1 s \<equiv> toEnvP s \<and>
-P3 s (\<lambda> s2'.  P12sub s2' ON_OFF_TIME'TIMEOUT (\<lambda> s1. getVarBool s1 enabled' = True) (\<lambda> s2. getVarBool s2 onOff' \<noteq> PRESSED')
- (\<lambda> s3. getVarBool s3 onOff' = PRESSED'))
-  (\<lambda> s2. getVarBool s2 roller' = False \<and> getVarBool s2 vibration' = False)"
+P2 s (\<lambda> s1 s2.  P12op s1 ON_OFF_TIME'TIMEOUT (\<lambda> s3. getVarBool s3 enabled' = True)  (\<lambda> s4. getVarBool s4 onOff' = PRESSED') \<and> getVarBool s2 onOff' \<noteq> PRESSED')
+ (\<lambda> s1 s2. getVarBool s2 roller' = False \<and> getVarBool s2 vibration' = False)
+"
 
 definition R8 where "R8 s \<equiv> toEnvP s \<and>
 (\<forall> s1 s2 s4. substate s1 s2 \<and> substate s2 s4 \<and> substate s4 s \<and> toEnvP s1 \<and> toEnvP s2 \<and> toEnvP s4 \<and> toEnvNum s1 s2 > ON_OFF_TIME'TIMEOUT  \<and> (getVarBool s1 enabled' = True) \<and>
@@ -43,10 +43,11 @@ definition R8 where "R8 s \<equiv> toEnvP s \<and>
 (\<forall> s5. toEnvP s5 \<and> substate s2 s5 \<and> substate s5 s4 \<longrightarrow> getVarBool s5 upper' = False) \<longrightarrow>
 getVarBool s4 up' = True)"
 
+
 definition R8_1 where "R8_1 s \<equiv> toEnvP s \<and>
-P6_1 s (\<lambda> s2. P12sub s2 ON_OFF_TIME'TIMEOUT (\<lambda> s1. getVarBool s1 enabled' = True) (\<lambda> s2'. getVarBool s2' onOff' \<noteq> PRESSED') (\<lambda> s3. getVarBool s3 onOff' = PRESSED'))
-(\<lambda> s4. getVarBool s4 up' = True)
-(\<lambda> s5. getVarBool s5 upper' = True)"
+P6 s (\<lambda> s3 s4. P12op s3 ON_OFF_TIME'TIMEOUT (\<lambda> s1. getVarBool s1 enabled' = True) (\<lambda> s2. getVarBool s2 onOff' = PRESSED') \<and> getVarBool s4 onOff' \<noteq> PRESSED')
+(\<lambda> s5. getVarBool s5 up' = True) (\<lambda> s6. getVarBool s6 upper' = True)"
+
 
 definition R9 where "R9 s \<equiv> toEnvP s \<and>
 P6 s (\<lambda> s1 s2. getVarBool s1 enabled' = True \<and> getVarBool s2 enabled' = False) (\<lambda> s3. getVarBool s3 up' = True) (\<lambda> s4. getVarBool s4 upper' = True)"
