Pattern6_Def.thy
@@ -27,9 +27,7 @@ lemma P6_rule: "P6 s0 A1 A2 A3 \<Longrightarrow> \<not> A3 s \<longrightarrow> A
   apply(unfold P6_def)
   by (smt (verit, best) One_nat_def add_is_1 substate_linear substate_toEnvNum_id toEnvNum3)
 
-lemma einv2req: "P6 s0 A1 A2 A3 \<Longrightarrow>  P6inv s0 A1 A3 \<Longrightarrow> A1 s0 s \<and> \<not> A3 s \<longrightarrow> A2 s \<Longrightarrow> toEnvP s0 \<and> toEnvP s \<and> substate s0 s \<and> toEnvNum s0 s = 1 \<Longrightarrow> P6 s A1 A2 A3"
-  apply(unfold P6_def P6inv_def)
-  by (smt (verit, ccfv_threshold) less_one nat_neq_iff not_add_less2 substate_linear substate_toEnvNum_id substate_trans toEnvNum3 toEnvNum_eq_imp_eq2)
+
 
 definition P6inv1 where "P6inv1 s w A1 A2 A3 \<equiv>
 \<forall>s1 s2 s3.
@@ -49,6 +47,23 @@ lemma einv2req1: "P6inv1 s w A1 A2 A3 \<Longrightarrow> P6 s A1 A2 A3"
   apply(unfold P6inv1_def P6_def)
   by auto
 
+definition P6_1inv1 where "P6_1inv1 s w A1 A2 A3 \<equiv>
+\<forall>s1 s2.
+   substate s1 s2 \<and>
+   substate s2 s \<and> toEnvP s1 \<and> toEnvP s2 \<and>  A1 s1 \<and> (\<forall>s3. toEnvP s3 \<and> substate s1 s3 \<and> substate s3 s2 \<longrightarrow> \<not> A3 s3) \<longrightarrow>
+   A2 s2 \<and> (w \<or> s2 \<noteq> s)"
+
+lemma P6_1inv1_rule: "P6_1inv1 s0 w1 A1 A2 A3 \<Longrightarrow>
+A1 s \<and> \<not> A3 s \<longrightarrow> A2 s \<and> w2 \<Longrightarrow>
+w1 \<and> A2 s0 \<and> \<not> A3 s \<longrightarrow> A2 s \<and> w2 \<Longrightarrow>
+ toEnvP s0 \<and> toEnvP s \<and> substate s0 s \<and> toEnvNum s0 s = 1 \<Longrightarrow> P6_1inv1 s w2 A1 A2 A3"
+  apply(unfold P6_1inv1_def)
+  by (smt (verit, ccfv_threshold) substate_noteq_imp_substate_of_pred substate_trans toEnvNum_eq_imp_eq2)
+
+lemma P6_1einv2req: "P6_1inv1 s w A1 A2 A3 \<Longrightarrow> P6_1 s A1 A2 A3"
+  apply(unfold P6_1inv1_def P6_1_def)
+  apply auto
+  done
 
 
 end
