MassageChair/Proofs_R8.thy
@@ -1,0 +1,124 @@
+theory Proofs_R8
+  imports Requirements ExtraInv_R8
+begin
+
+definition inv8 where "inv8 s \<equiv> extraInv s \<and> R8_1 s"
+
+theorem "VC1 inv8 s0"
+  apply(unfold VC1_def inv8_def R8_1_def P6_def P12op_def)
+  using extra1 VC1_def apply auto
+  done
+
+theorem  "VC182 inv8 env s0 onOff'value startButton'value rollerButton'value vibrationButton'value buttonUp'value buttonDown'value
+ upper'value lower'value"
+  apply(unfold VC182_def inv8_def R8_1_def)
+   apply(rule impI)
+  apply(rule conjI)
+  using extra182 apply(auto simp add: VC182_def)[1] 
+  apply(rule conjI)
+  apply simp
+  apply(unfold extraInv_def commonExtraInv_def)
+  apply(erule conjE)+
+  apply simp
+  done
+
+theorem  "VC362 inv8 env s0 onOff'value startButton'value rollerButton'value vibrationButton'value buttonUp'value buttonDown'value
+ upper'value lower'value"
+  apply(unfold VC362_def inv8_def R8_1_def)
+   apply(rule impI)
+  apply(rule conjI)
+  using extra362 apply(auto simp add: VC362_def)[1] 
+  apply(rule conjI)
+  apply simp
+  apply(unfold extraInv_def commonExtraInv_def)
+  apply(erule conjE)+
+  apply simp
+  done
+
+theorem  "VC542 inv8 env s0 onOff'value startButton'value rollerButton'value vibrationButton'value buttonUp'value buttonDown'value
+ upper'value lower'value"
+  apply(unfold VC542_def inv8_def R8_1_def)
+   apply(rule impI)
+  apply(rule conjI)
+  using extra542 apply(auto simp add: VC542_def)[1] 
+  apply(rule conjI)
+  apply simp
+  apply(unfold extraInv_def commonExtraInv_def)
+  apply(erule conjE)+
+  apply simp
+  done
+
+theorem  "VC722 inv8 env s0 onOff'value startButton'value rollerButton'value vibrationButton'value buttonUp'value buttonDown'value
+ upper'value lower'value"
+  apply(unfold VC722_def inv8_def R8_1_def)
+   apply(rule impI)
+  apply(rule context_conjI)
+  using extra722 apply(auto simp add: VC722_def)[1]
+  apply(rule conjI)
+  apply simp
+  apply(unfold extraInv_def commonExtraInv_def)
+  apply(erule conjE)+
+  apply simp
+  apply(rule Pattern6_Def.einv2req1)
+  apply auto
+  done
+
+theorem  "VC902 inv8 env s0 onOff'value startButton'value rollerButton'value vibrationButton'value buttonUp'value buttonDown'value
+ upper'value lower'value"
+  apply(unfold VC902_def inv8_def R8_1_def)
+   apply(rule impI)
+  apply(rule context_conjI)
+  using extra902 apply(auto simp add: VC902_def)[1]
+  apply(rule conjI)
+  apply simp
+  apply(unfold extraInv_def commonExtraInv_def)
+  apply(erule conjE)+
+  apply simp
+  done
+
+theorem  "VC1262 inv8 env s0 onOff'value startButton'value rollerButton'value vibrationButton'value buttonUp'value buttonDown'value
+ upper'value lower'value"
+  apply(unfold VC1262_def inv8_def R8_1_def)
+   apply(rule impI)
+  apply(rule context_conjI)
+  using extra1262 apply(auto simp add: VC1262_def)[1]
+  apply(rule conjI)
+  apply simp
+  apply(unfold extraInv_def commonExtraInv_def)
+  apply(erule conjE)+
+  apply simp
+  apply(rule Pattern6_Def.einv2req1)
+  apply auto
+  done
+
+theorem  "VC1622 inv8 env s0 onOff'value startButton'value rollerButton'value vibrationButton'value buttonUp'value buttonDown'value
+ upper'value lower'value"
+  apply(unfold VC1622_def inv8_def R8_1_def)
+   apply(rule impI)
+  apply(rule context_conjI)
+  using extra1622 apply(auto simp add: VC1622_def)[1]
+  apply(rule conjI)
+  apply simp
+  apply(unfold extraInv_def commonExtraInv_def)
+  apply(erule conjE)+
+  apply simp
+  apply(rule Pattern6_Def.einv2req1)
+  apply auto
+  done
+
+theorem  "VC1802 inv8 env s0 onOff'value startButton'value rollerButton'value vibrationButton'value buttonUp'value buttonDown'value
+ upper'value lower'value"
+  apply(unfold VC1802_def inv8_def R8_1_def)
+   apply(rule impI)
+  apply(rule context_conjI)
+  using extra1802 apply(auto simp add: VC1802_def)[1]
+  apply(rule conjI)
+  apply simp
+  apply(unfold extraInv_def commonExtraInv_def)
+  apply(erule conjE)+
+  apply simp
+   apply(rule Pattern6_Def.einv2req1)
+  apply auto
+  done
+
+end
