Pattern2_Def.thy
@@ -9,7 +9,7 @@ definition P2ex where "P2ex s A \<equiv>
 \<exists> s1. consecutive s1 s \<and> A s1 s"
 
 definition P2 where  "P2 s A1 A2 \<equiv> toEnvP s \<and>
-(\<forall> s1 s2. consecutive s1 s2 \<and> A1 s1 s2 \<longrightarrow> A2 s1 s2)"
+(\<forall> s1 s2. consecutive s1 s2 \<and> substate s2 s \<and> A1 s1 s2 \<longrightarrow> A2 s1 s2)"
 
 lemma P2all_rule: "consecutive s0 s \<Longrightarrow> P2all s A = A s0 s"
   apply(unfold consecutive_def P2all_def)
@@ -21,7 +21,8 @@ lemma P2ex_rule: "consecutive s0 s \<Longrightarrow> P2ex s A = A s0 s"
 
 lemma P2_rule: "consecutive s0 s \<Longrightarrow> P2 s0 A1 A2 \<Longrightarrow> (consecutive s0 s \<Longrightarrow> A1 s0 s \<longrightarrow> A2 s0 s) \<Longrightarrow> P2 s A1 A2"
   apply simp
-  apply(unfold P2_def)
-  using consecutive_def by blast
+  apply(unfold P2_def consecutive_def)
+  by (metis One_nat_def substate_noteq_imp_substate_of_pred toEnvNum_eq_imp_eq2)
 
 end
+  
